LeanCats/Denote.lean
@@ -1,0 +1,13 @@
+import Mathlib.Data.Set.Basic
+
+def State : Type :=
+  String → Nat
+
+def Identity {α : Type} : Set (α × α) :=
+  {ab | ab.fst = ab.snd }
+
+inductive Stmt : Type where
+  | assign : String -> (State -> Nat) -> Stmt
+  | seq : Stmt -> Stmt -> Stmt
+
+inductive CatDenote ->
